
@prefix tree: <https://w3id.org/tree#> .
@prefix ldes: <https://w3id.org/ldes#> .
@prefix dc: <http://purl.org/dc/terms/> .
@prefix sh: <http://www.w3.org/ns/shacl#> .
@prefix xsd: <http://www.w3.org/2001/XMLSchema#> .
@prefix skos: <http://www.w3.org/2004/02/skos/core#> .
@prefix dcat: <http://www.w3.org/ns/dcat#> .

<http://vocab.nerc.ac.uk/ldes/P02/2016-01-01%2000%3A00%3A00_2016-12-31%2000%3A00%3A00>
    a tree:Node ;
    
    tree:relation [ tree:node <http://vocab.nerc.ac.uk/ldes/P02/2015-12-31%2000%3A00%3A00_2016-01-01%2000%3A00%3A00> ] ;
    
    ldes:retentionPolicy [
        a ldes:LatestVersionSubset ;
        ldes:amount 15 ;
        ldes:versionKey ( dc:isVersionOf )
    ] .

<http://vocab.nerc.ac.uk/ldes/P02>
  a ldes:EventStream ;
  tree:shape [
    a sh:NodeShape ;
    sh:nodeKind sh:IRI ;
    sh:property [
      sh:datatype xsd:string ;
      sh:minCount 1 ;
      sh:path dc:isVersionOf
    ],
    [
      sh:datatype xsd:dateTime ;
      sh:minCount 1 ;
      sh:path dc:modified
    ],
    [
      sh:datatype xsd:string ;
      sh:minCount 1 ;
      sh:path skos:altLabel
    ],
    [
      sh:datatype xsd:string ;
      sh:minCount 1 ;
      sh:path skos:definition
    ],
    [
      sh:datatype xsd:string ;
      sh:minCount 1 ;
      sh:path skos:notation
    ];
    sh:targetClass skos:Concept
  ] ;
  tree:view <http://vocab.nerc.ac.uk/ldes/P02/2016-01-01%2000%3A00%3A00_2016-12-31%2000%3A00%3A00> ;
  .

<http://vocab.nerc.ac.uk/ldes/P02> tree:member <http://vocab.nerc.ac.uk/collection/P02/current/BCMT/5/> .
<http://vocab.nerc.ac.uk/collection/P02/current/BCMT/5/>
    a skos:Concept ;
    dc:isVersionOf "http://vocab.nerc.ac.uk/collection/P02/current/BCMT/".
<http://vocab.nerc.ac.uk/collection/P02/current/BCMT/>
    dcat:modified "2016-10-04 14:27:37.0"^^xsd:dateTime ;
    skos:altLabel "Met_Biota" ;
    skos:definition "Metal concentrations in either whole organisms or their constituent parts." ;
    skos:notation "SDN:P02::BCMT" .
    
<http://vocab.nerc.ac.uk/ldes/P02> tree:member <http://vocab.nerc.ac.uk/collection/P02/current/CCPW/3/> .
<http://vocab.nerc.ac.uk/collection/P02/current/CCPW/3/>
    a skos:Concept ;
    dc:isVersionOf "http://vocab.nerc.ac.uk/collection/P02/current/CCPW/".
<http://vocab.nerc.ac.uk/collection/P02/current/CCPW/>
    dcat:modified "2016-06-02 15:14:26.0"^^xsd:dateTime ;
    skos:altLabel "SedPoreWat_CarbChem" ;
    skos:definition "Carbonate system parameters (DIC/TCO2, pH, alkalinity, pCO2) in sediment pore waters" ;
    skos:notation "SDN:P02::CCPW" .
    
<http://vocab.nerc.ac.uk/ldes/P02> tree:member <http://vocab.nerc.ac.uk/collection/P02/current/INVD/1/> .
<http://vocab.nerc.ac.uk/collection/P02/current/INVD/1/>
    a skos:Concept ;
    dc:isVersionOf "http://vocab.nerc.ac.uk/collection/P02/current/INVD/".
<http://vocab.nerc.ac.uk/collection/P02/current/INVD/>
    dcat:modified "2016-05-19 16:45:42.0"^^xsd:dateTime ;
    skos:altLabel "InvasiveSpecies" ;
    skos:definition "Parameters used to characterize and monitor biological invasion by non-native organisms." ;
    skos:notation "SDN:P02::INVD" .
    
<http://vocab.nerc.ac.uk/ldes/P02> tree:member <http://vocab.nerc.ac.uk/collection/P02/current/GPIG/3/> .
<http://vocab.nerc.ac.uk/collection/P02/current/GPIG/3/>
    a skos:Concept ;
    dc:isVersionOf "http://vocab.nerc.ac.uk/collection/P02/current/GPIG/".
<http://vocab.nerc.ac.uk/collection/P02/current/GPIG/>
    dcat:modified "2016-02-16 15:55:29.0"^^xsd:dateTime ;
    skos:altLabel "GutPig" ;
    skos:definition "Parameters identifying or quantifying zooplankton gut pigments" ;
    skos:notation "SDN:P02::GPIG" .
    
<http://vocab.nerc.ac.uk/ldes/P02> tree:member <http://vocab.nerc.ac.uk/collection/P02/current/STGC/1/> .
<http://vocab.nerc.ac.uk/collection/P02/current/STGC/1/>
    a skos:Concept ;
    dc:isVersionOf "http://vocab.nerc.ac.uk/collection/P02/current/STGC/".
<http://vocab.nerc.ac.uk/collection/P02/current/STGC/>
    dcat:modified "2016-02-16 15:44:14.0"^^xsd:dateTime ;
    skos:altLabel "StomachGutContents" ;
    skos:definition "Parameters that characterize or quantify the contents of the stomach and gut of an animal or group of animals." ;
    skos:notation "SDN:P02::STGC" .
    
