
@prefix tree: <https://w3id.org/tree#> .
@prefix ldes: <https://w3id.org/ldes#> .
@prefix dc: <http://purl.org/dc/terms/> .
@prefix sh: <http://www.w3.org/ns/shacl#> .
@prefix xsd: <http://www.w3.org/2001/XMLSchema#> .
@prefix skos: <http://www.w3.org/2004/02/skos/core#> .
@prefix dcat: <http://www.w3.org/ns/dcat#> .

<http://vocab.nerc.ac.uk/ldes/P02/2015-01-01%2000%3A00%3A00_2015-12-31%2000%3A00%3A00>
    a tree:Node ;
    
    tree:relation [ tree:node <http://vocab.nerc.ac.uk/ldes/P02/2014-12-31%2000%3A00%3A00_2015-01-01%2000%3A00%3A00> ] ;
    
    ldes:retentionPolicy [
        a ldes:LatestVersionSubset ;
        ldes:amount 15 ;
        ldes:versionKey ( dc:isVersionOf )
    ] .

<http://vocab.nerc.ac.uk/ldes/P02>
  a ldes:EventStream ;
  tree:shape [
    a sh:NodeShape ;
    sh:nodeKind sh:IRI ;
    sh:property [
      sh:datatype xsd:string ;
      sh:minCount 1 ;
      sh:path dc:isVersionOf
    ],
    [
      sh:datatype xsd:dateTime ;
      sh:minCount 1 ;
      sh:path dc:modified
    ],
    [
      sh:datatype xsd:string ;
      sh:minCount 1 ;
      sh:path skos:altLabel
    ],
    [
      sh:datatype xsd:string ;
      sh:minCount 1 ;
      sh:path skos:definition
    ],
    [
      sh:datatype xsd:string ;
      sh:minCount 1 ;
      sh:path skos:notation
    ];
    sh:targetClass skos:Concept
  ] ;
  tree:view <http://vocab.nerc.ac.uk/ldes/P02/2015-01-01%2000%3A00%3A00_2015-12-31%2000%3A00%3A00> ;
  .

<http://vocab.nerc.ac.uk/ldes/P02> tree:member <http://vocab.nerc.ac.uk/collection/P02/current/PHLT/1/> .
<http://vocab.nerc.ac.uk/collection/P02/current/PHLT/1/>
    a skos:Concept ;
    dc:isVersionOf "http://vocab.nerc.ac.uk/collection/P02/current/PHLT/".
<http://vocab.nerc.ac.uk/collection/P02/current/PHLT/>
    dcat:modified "2015-11-16 13:22:28.0"^^xsd:dateTime ;
    skos:altLabel "Raw_pH_output" ;
    skos:definition "Raw pH parameter output from any type of pH sensor." ;
    skos:notation "SDN:P02::PHLT" .
    
<http://vocab.nerc.ac.uk/ldes/P02> tree:member <http://vocab.nerc.ac.uk/collection/P02/current/CARO/3/> .
<http://vocab.nerc.ac.uk/collection/P02/current/CARO/3/>
    a skos:Concept ;
    dc:isVersionOf "http://vocab.nerc.ac.uk/collection/P02/current/CARO/".
<http://vocab.nerc.ac.uk/collection/P02/current/CARO/>
    dcat:modified "2015-09-08 09:02:34.0"^^xsd:dateTime ;
    skos:altLabel "WC_CarotFlavPig" ;
    skos:definition "" ;
    skos:notation "SDN:P02::CARO" .
    
<http://vocab.nerc.ac.uk/ldes/P02> tree:member <http://vocab.nerc.ac.uk/collection/P02/current/IALZ/2/> .
<http://vocab.nerc.ac.uk/collection/P02/current/IALZ/2/>
    a skos:Concept ;
    dc:isVersionOf "http://vocab.nerc.ac.uk/collection/P02/current/IALZ/".
<http://vocab.nerc.ac.uk/collection/P02/current/IALZ/>
    dcat:modified "2015-04-08 15:27:34.0"^^xsd:dateTime ;
    skos:altLabel "Littoral_TaxInsectWormAFDW" ;
    skos:definition "Insect (Class Insecta) and earthworm (Subclass Oligochaeta) ash-free dry weight biomass per unit area of the littoral zone (between spring tide high and low water) parameters." ;
    skos:notation "SDN:P02::IALZ" .
    
<http://vocab.nerc.ac.uk/ldes/P02> tree:member <http://vocab.nerc.ac.uk/collection/P02/current/INLZ/2/> .
<http://vocab.nerc.ac.uk/collection/P02/current/INLZ/2/>
    a skos:Concept ;
    dc:isVersionOf "http://vocab.nerc.ac.uk/collection/P02/current/INLZ/".
<http://vocab.nerc.ac.uk/collection/P02/current/INLZ/>
    dcat:modified "2015-04-08 15:26:45.0"^^xsd:dateTime ;
    skos:altLabel "InsWorm_Tax_Litabund" ;
    skos:definition "Insect (Class Insecta) and earthworm (Subclass Oligochaeta) abundance per unit area of the littoral zone (between spring tide high and low water) parameters." ;
    skos:notation "SDN:P02::INLZ" .
    
<http://vocab.nerc.ac.uk/ldes/P02> tree:member <http://vocab.nerc.ac.uk/collection/P02/current/MFAZ/2/> .
<http://vocab.nerc.ac.uk/collection/P02/current/MFAZ/2/>
    a skos:Concept ;
    dc:isVersionOf "http://vocab.nerc.ac.uk/collection/P02/current/MFAZ/".
<http://vocab.nerc.ac.uk/collection/P02/current/MFAZ/>
    dcat:modified "2015-04-08 15:23:44.0"^^xsd:dateTime ;
    skos:altLabel "Littoral_TaxZoobenthAFDW" ;
    skos:definition "Any zoobenthos ash-free dry weight biomass per unit area of the littoral zone (between spring tide high and low water) parameters that are not fish or terrestrial animals (insecta/oligochaeta)" ;
    skos:notation "SDN:P02::MFAZ" .
    
<http://vocab.nerc.ac.uk/ldes/P02> tree:member <http://vocab.nerc.ac.uk/collection/P02/current/MFLZ/2/> .
<http://vocab.nerc.ac.uk/collection/P02/current/MFLZ/2/>
    a skos:Concept ;
    dc:isVersionOf "http://vocab.nerc.ac.uk/collection/P02/current/MFLZ/".
<http://vocab.nerc.ac.uk/collection/P02/current/MFLZ/>
    dcat:modified "2015-04-08 15:22:45.0"^^xsd:dateTime ;
    skos:altLabel "Zoobenth_Tax_Litabund" ;
    skos:definition "Any zoobenthos abundance per unit area of the littoral zone (between spring tide high and low water) parameters that are not fish or terrestrial animals (insecta/oligochaeta)" ;
    skos:notation "SDN:P02::MFLZ" .
    
<http://vocab.nerc.ac.uk/ldes/P02> tree:member <http://vocab.nerc.ac.uk/collection/P02/current/BEPP/1/> .
<http://vocab.nerc.ac.uk/collection/P02/current/BEPP/1/>
    a skos:Concept ;
    dc:isVersionOf "http://vocab.nerc.ac.uk/collection/P02/current/BEPP/".
<http://vocab.nerc.ac.uk/collection/P02/current/BEPP/>
    dcat:modified "2015-02-03 10:19:46.0"^^xsd:dateTime ;
    skos:altLabel "Ben_PrimaryProd" ;
    skos:definition "Parameters associated with the quantification of primary production by plants living on (e.g. corals, seaweed and seagrass) or in (e.g. benthic diatoms) the seabed.  Primary production is defined as the fixation of carbon dioxide into either organic or inorganic carbon by living entities and so includes photosynthesis and calcification." ;
    skos:notation "SDN:P02::BEPP" .
    
