
@prefix tree: <https://w3id.org/tree#> .
@prefix ldes: <https://w3id.org/ldes#> .
@prefix dc: <http://purl.org/dc/terms/> .
@prefix sh: <http://www.w3.org/ns/shacl#> .
@prefix xsd: <http://www.w3.org/2001/XMLSchema#> .
@prefix skos: <http://www.w3.org/2004/02/skos/core#> .
@prefix dcat: <http://www.w3.org/ns/dcat#> .

<http://vocab.nerc.ac.uk/ldes/P02/2019-01-01%2000%3A00%3A00_2019-12-31%2000%3A00%3A00>
    a tree:Node ;
    
    tree:relation [ tree:node <http://vocab.nerc.ac.uk/ldes/P02/2018-12-31%2000%3A00%3A00_2019-01-01%2000%3A00%3A00> ] ;
    
    ldes:retentionPolicy [
        a ldes:LatestVersionSubset ;
        ldes:amount 1 ;
        ldes:versionKey ( dc:isVersionOf )
    ] .

<http://vocab.nerc.ac.uk/ldes/P02>
  a ldes:EventStream ;
  tree:shape [
    a sh:NodeShape ;
    sh:nodeKind sh:IRI ;
    sh:property [
      sh:datatype xsd:string ;
      sh:minCount 1 ;
      sh:path dc:isVersionOf
    ],
    [
      sh:datatype xsd:dateTime ;
      sh:minCount 1 ;
      sh:path dc:modified
    ],
    [
      sh:datatype xsd:string ;
      sh:minCount 1 ;
      sh:path skos:altLabel
    ],
    [
      sh:datatype xsd:string ;
      sh:minCount 1 ;
      sh:path skos:definition
    ],
    [
      sh:datatype xsd:string ;
      sh:minCount 1 ;
      sh:path skos:notation
    ];
    sh:targetClass skos:Concept
  ] ;
  tree:view <http://vocab.nerc.ac.uk/ldes/P02/2019-01-01%2000%3A00%3A00_2019-12-31%2000%3A00%3A00> ;
  .

<http://vocab.nerc.ac.uk/ldes/P02> tree:member <http://vocab.nerc.ac.uk/collection/P02/current/FADS/1/> .
<http://vocab.nerc.ac.uk/collection/P02/current/FADS/1/>
    a skos:Concept ;
    dc:isVersionOf "http://vocab.nerc.ac.uk/collection/P02/current/FADS/".
<http://vocab.nerc.ac.uk/collection/P02/current/FADS/>
    dcat:modified "2019-07-26 11:05:38.0"^^xsd:dateTime ;
    skos:altLabel "FAD usage statistics" ;
    skos:definition "Parameters describing usage of Fish Aggregating Devices (FAD) in fisheries (particularly purse seine tuna fisheries)." ;
    skos:notation "SDN:P02::FADS" .
<http://vocab.nerc.ac.uk/ldes/P02> tree:member <http://vocab.nerc.ac.uk/collection/P02/current/ATPX/2/> .
<http://vocab.nerc.ac.uk/collection/P02/current/ATPX/2/>
    a skos:Concept ;
    dc:isVersionOf "http://vocab.nerc.ac.uk/collection/P02/current/ATPX/".
<http://vocab.nerc.ac.uk/collection/P02/current/ATPX/>
    dcat:modified "2019-06-13 08:54:58.0"^^xsd:dateTime ;
    skos:altLabel "Aden_WC" ;
    skos:definition "Concentrations of adenylates (ADP, ATP etc) in all phases of the water column" ;
    skos:notation "SDN:P02::ATPX" .
<http://vocab.nerc.ac.uk/ldes/P02> tree:member <http://vocab.nerc.ac.uk/collection/P02/current/GP025/3/> .
<http://vocab.nerc.ac.uk/collection/P02/current/GP025/3/>
    a skos:Concept ;
    dc:isVersionOf "http://vocab.nerc.ac.uk/collection/P02/current/GP025/".
<http://vocab.nerc.ac.uk/collection/P02/current/GP025/>
    dcat:modified "2019-05-31 19:13:30.0"^^xsd:dateTime ;
    skos:altLabel "SealRepr" ;
    skos:definition "Parameters related to the reproduction of true seals (Phocidae), eared seals (Otariidae) and walruses (Odobenidae)." ;
    skos:notation "SDN:P02::GP025" .
<http://vocab.nerc.ac.uk/ldes/P02> tree:member <http://vocab.nerc.ac.uk/collection/P02/current/SEBH/3/> .
<http://vocab.nerc.ac.uk/collection/P02/current/SEBH/3/>
    a skos:Concept ;
    dc:isVersionOf "http://vocab.nerc.ac.uk/collection/P02/current/SEBH/".
<http://vocab.nerc.ac.uk/collection/P02/current/SEBH/>
    dcat:modified "2019-05-31 19:13:30.0"^^xsd:dateTime ;
    skos:altLabel "Seal_Behav" ;
    skos:definition "Parameters describing the actions or reactions, usually in response to the environment, of true seals (Phocidae), eared seals (Otariidae) and walruses (Odobenidae)." ;
    skos:notation "SDN:P02::SEBH" .
<http://vocab.nerc.ac.uk/ldes/P02> tree:member <http://vocab.nerc.ac.uk/collection/P02/current/SEMP/3/> .
<http://vocab.nerc.ac.uk/collection/P02/current/SEMP/3/>
    a skos:Concept ;
    dc:isVersionOf "http://vocab.nerc.ac.uk/collection/P02/current/SEMP/".
<http://vocab.nerc.ac.uk/collection/P02/current/SEMP/>
    dcat:modified "2019-05-31 19:13:30.0"^^xsd:dateTime ;
    skos:altLabel "Seal_Morph_Phys" ;
    skos:definition "Parameters describing the size, shape or physiological activity including disease and parasite infection status of true seals (Phocidae), eared seals (Otariidae) and walruses (Odobenidae)." ;
    skos:notation "SDN:P02::SEMP" .
<http://vocab.nerc.ac.uk/ldes/P02> tree:member <http://vocab.nerc.ac.uk/collection/P02/current/SEMO/4/> .
<http://vocab.nerc.ac.uk/collection/P02/current/SEMO/4/>
    a skos:Concept ;
    dc:isVersionOf "http://vocab.nerc.ac.uk/collection/P02/current/SEMO/".
<http://vocab.nerc.ac.uk/collection/P02/current/SEMO/>
    dcat:modified "2019-05-31 19:13:30.0"^^xsd:dateTime ;
    skos:altLabel "Seal_Mort" ;
    skos:definition "Parameters describing the causes and rate of mortality of true seals (Phocidae), eared seals (Otariidae) and walruses (Odobenidae)." ;
    skos:notation "SDN:P02::SEMO" .
