
@prefix tree: <https://w3id.org/tree#> .
@prefix ldes: <https://w3id.org/ldes#> .
@prefix dc: <http://purl.org/dc/terms/> .
@prefix sh: <http://www.w3.org/ns/shacl#> .
@prefix xsd: <http://www.w3.org/2001/XMLSchema#> .
@prefix skos: <http://www.w3.org/2004/02/skos/core#> .
@prefix dcat: <http://www.w3.org/ns/dcat#> .

<http://vocab.nerc.ac.uk/ldes/P03/2017-01-01%2000%3A00%3A00_2017-12-31%2000%3A00%3A00>
    a tree:Node ;
    
    tree:relation [ tree:node <http://vocab.nerc.ac.uk/ldes/P03/2016-12-31%2000%3A00%3A00_2017-01-01%2000%3A00%3A00> ] ;
    
    ldes:retentionPolicy [
        a ldes:LatestVersionSubset ;
        ldes:amount 15 ;
        ldes:versionKey ( dc:isVersionOf )
    ] .

<http://vocab.nerc.ac.uk/ldes/P03>
  a ldes:EventStream ;
  tree:shape [
    a sh:NodeShape ;
    sh:nodeKind sh:IRI ;
    sh:property [
      sh:datatype xsd:string ;
      sh:minCount 1 ;
      sh:path dc:isVersionOf
    ],
    [
      sh:datatype xsd:dateTime ;
      sh:minCount 1 ;
      sh:path dc:modified
    ],
    [
      sh:datatype xsd:string ;
      sh:minCount 1 ;
      sh:path skos:altLabel
    ],
    [
      sh:datatype xsd:string ;
      sh:minCount 1 ;
      sh:path skos:definition
    ],
    [
      sh:datatype xsd:string ;
      sh:minCount 1 ;
      sh:path skos:notation
    ];
    sh:targetClass skos:Concept
  ] ;
  tree:view <http://vocab.nerc.ac.uk/ldes/P03/2017-01-01%2000%3A00%3A00_2017-12-31%2000%3A00%3A00> ;
  .

<http://vocab.nerc.ac.uk/ldes/P03> tree:member <http://vocab.nerc.ac.uk/collection/P03/current/INAZ/1/> .
<http://vocab.nerc.ac.uk/collection/P03/current/INAZ/1/>
    a skos:Concept ;
    dc:isVersionOf "http://vocab.nerc.ac.uk/collection/P03/current/INAZ/".
<http://vocab.nerc.ac.uk/collection/P03/current/INAZ/>
    dcat:modified "2017-05-02 13:13:32.0"^^xsd:dateTime ;
    skos:altLabel "Inapplicable" ;
    skos:definition "There is no appropriate value." ;
    skos:notation "SDN:P03::INAZ" .
    
<http://vocab.nerc.ac.uk/ldes/P03> tree:member <http://vocab.nerc.ac.uk/collection/P03/current/H001/2/> .
<http://vocab.nerc.ac.uk/collection/P03/current/H001/2/>
    a skos:Concept ;
    dc:isVersionOf "http://vocab.nerc.ac.uk/collection/P03/current/H001/".
<http://vocab.nerc.ac.uk/collection/P03/current/H001/>
    dcat:modified "2017-02-02 14:38:40.0"^^xsd:dateTime ;
    skos:altLabel "" ;
    skos:definition "Parameters describing the abundance, nature and impact of material added to the environment by the activities of man." ;
    skos:notation "SDN:P03::H001" .
    
<http://vocab.nerc.ac.uk/ldes/P03> tree:member <http://vocab.nerc.ac.uk/collection/P03/current/H005/2/> .
<http://vocab.nerc.ac.uk/collection/P03/current/H005/2/>
    a skos:Concept ;
    dc:isVersionOf "http://vocab.nerc.ac.uk/collection/P03/current/H005/".
<http://vocab.nerc.ac.uk/collection/P03/current/H005/>
    dcat:modified "2017-02-02 14:38:40.0"^^xsd:dateTime ;
    skos:altLabel "" ;
    skos:definition "Parameters quantifying the level of any type of human activity, generally in the context of environmental considerations" ;
    skos:notation "SDN:P03::H005" .
    
<http://vocab.nerc.ac.uk/ldes/P03> tree:member <http://vocab.nerc.ac.uk/collection/P03/current/H006/1/> .
<http://vocab.nerc.ac.uk/collection/P03/current/H006/1/>
    a skos:Concept ;
    dc:isVersionOf "http://vocab.nerc.ac.uk/collection/P03/current/H006/".
<http://vocab.nerc.ac.uk/collection/P03/current/H006/>
    dcat:modified "2017-02-02 14:38:40.0"^^xsd:dateTime ;
    skos:altLabel "" ;
    skos:definition "Datasets related to the process or industry of farming aquatic animal and plants." ;
    skos:notation "SDN:P03::H006" .
    
<http://vocab.nerc.ac.uk/ldes/P03> tree:member <http://vocab.nerc.ac.uk/collection/P03/current/H007/1/> .
<http://vocab.nerc.ac.uk/collection/P03/current/H007/1/>
    a skos:Concept ;
    dc:isVersionOf "http://vocab.nerc.ac.uk/collection/P03/current/H007/".
<http://vocab.nerc.ac.uk/collection/P03/current/H007/>
    dcat:modified "2017-02-02 14:38:40.0"^^xsd:dateTime ;
    skos:altLabel "" ;
    skos:definition "Datasets related to the process of managing aquatic and coastal environments." ;
    skos:notation "SDN:P03::H007" .
    
<http://vocab.nerc.ac.uk/ldes/P03> tree:member <http://vocab.nerc.ac.uk/collection/P03/current/H008/1/> .
<http://vocab.nerc.ac.uk/collection/P03/current/H008/1/>
    a skos:Concept ;
    dc:isVersionOf "http://vocab.nerc.ac.uk/collection/P03/current/H008/".
<http://vocab.nerc.ac.uk/collection/P03/current/H008/>
    dcat:modified "2017-02-02 14:38:40.0"^^xsd:dateTime ;
    skos:altLabel "" ;
    skos:definition "Datasets related to the process or industry of deploying and maintaining communication and power cables." ;
    skos:notation "SDN:P03::H008" .
    
<http://vocab.nerc.ac.uk/ldes/P03> tree:member <http://vocab.nerc.ac.uk/collection/P03/current/H009/1/> .
<http://vocab.nerc.ac.uk/collection/P03/current/H009/1/>
    a skos:Concept ;
    dc:isVersionOf "http://vocab.nerc.ac.uk/collection/P03/current/H009/".
<http://vocab.nerc.ac.uk/collection/P03/current/H009/>
    dcat:modified "2017-02-02 14:38:40.0"^^xsd:dateTime ;
    skos:altLabel "" ;
    skos:definition "Datasets related to the process of managing cultural and historical artifacts." ;
    skos:notation "SDN:P03::H009" .
    
<http://vocab.nerc.ac.uk/ldes/P03> tree:member <http://vocab.nerc.ac.uk/collection/P03/current/H010/1/> .
<http://vocab.nerc.ac.uk/collection/P03/current/H010/1/>
    a skos:Concept ;
    dc:isVersionOf "http://vocab.nerc.ac.uk/collection/P03/current/H010/".
<http://vocab.nerc.ac.uk/collection/P03/current/H010/>
    dcat:modified "2017-02-02 14:38:40.0"^^xsd:dateTime ;
    skos:altLabel "" ;
    skos:definition "Datasets related to the process or industry of electrical power generation." ;
    skos:notation "SDN:P03::H010" .
    
<http://vocab.nerc.ac.uk/ldes/P03> tree:member <http://vocab.nerc.ac.uk/collection/P03/current/H011/1/> .
<http://vocab.nerc.ac.uk/collection/P03/current/H011/1/>
    a skos:Concept ;
    dc:isVersionOf "http://vocab.nerc.ac.uk/collection/P03/current/H011/".
<http://vocab.nerc.ac.uk/collection/P03/current/H011/>
    dcat:modified "2017-02-02 14:38:40.0"^^xsd:dateTime ;
    skos:altLabel "" ;
    skos:definition "Datasets related to the process or industry of locating and extracting hydrocarbon compounds from underground sources." ;
    skos:notation "SDN:P03::H011" .
    
<http://vocab.nerc.ac.uk/ldes/P03> tree:member <http://vocab.nerc.ac.uk/collection/P03/current/H012/1/> .
<http://vocab.nerc.ac.uk/collection/P03/current/H012/1/>
    a skos:Concept ;
    dc:isVersionOf "http://vocab.nerc.ac.uk/collection/P03/current/H012/".
<http://vocab.nerc.ac.uk/collection/P03/current/H012/>
    dcat:modified "2017-02-02 14:38:40.0"^^xsd:dateTime ;
    skos:altLabel "" ;
    skos:definition "Datasets related to the process or industry of locating and extracting coal or other minerals." ;
    skos:notation "SDN:P03::H012" .
    
<http://vocab.nerc.ac.uk/ldes/P03> tree:member <http://vocab.nerc.ac.uk/collection/P03/current/H013/1/> .
<http://vocab.nerc.ac.uk/collection/P03/current/H013/1/>
    a skos:Concept ;
    dc:isVersionOf "http://vocab.nerc.ac.uk/collection/P03/current/H013/".
<http://vocab.nerc.ac.uk/collection/P03/current/H013/>
    dcat:modified "2017-02-02 14:38:40.0"^^xsd:dateTime ;
    skos:altLabel "" ;
    skos:definition "Datasets related to the process or industry of deploying and maintaining pipelines." ;
    skos:notation "SDN:P03::H013" .
    
<http://vocab.nerc.ac.uk/ldes/P03> tree:member <http://vocab.nerc.ac.uk/collection/P03/current/H014/1/> .
<http://vocab.nerc.ac.uk/collection/P03/current/H014/1/>
    a skos:Concept ;
    dc:isVersionOf "http://vocab.nerc.ac.uk/collection/P03/current/H014/".
<http://vocab.nerc.ac.uk/collection/P03/current/H014/>
    dcat:modified "2017-02-02 14:38:40.0"^^xsd:dateTime ;
    skos:altLabel "" ;
    skos:definition "Datasets related to the process or industry of extracting salt from saltwater." ;
    skos:notation "SDN:P03::H014" .
    
<http://vocab.nerc.ac.uk/ldes/P03> tree:member <http://vocab.nerc.ac.uk/collection/P03/current/H015/1/> .
<http://vocab.nerc.ac.uk/collection/P03/current/H015/1/>
    a skos:Concept ;
    dc:isVersionOf "http://vocab.nerc.ac.uk/collection/P03/current/H015/".
<http://vocab.nerc.ac.uk/collection/P03/current/H015/>
    dcat:modified "2017-02-02 14:38:40.0"^^xsd:dateTime ;
    skos:altLabel "" ;
    skos:definition "Datasets related to the process or industry of tourism including activities and facilities or installations." ;
    skos:notation "SDN:P03::H015" .
    
<http://vocab.nerc.ac.uk/ldes/P03> tree:member <http://vocab.nerc.ac.uk/collection/P03/current/H016/1/> .
<http://vocab.nerc.ac.uk/collection/P03/current/H016/1/>
    a skos:Concept ;
    dc:isVersionOf "http://vocab.nerc.ac.uk/collection/P03/current/H016/".
<http://vocab.nerc.ac.uk/collection/P03/current/H016/>
    dcat:modified "2017-02-02 14:38:40.0"^^xsd:dateTime ;
    skos:altLabel "" ;
    skos:definition "Datasets related to the process or industry of transport including activities and facilities or installations." ;
    skos:notation "SDN:P03::H016" .
    
